ha2_refl.v
@@ -48,6 +48,16 @@ Fixpoint n_tm (n : nat) : tm :=
   | S n => Succ (n_tm n)
   end.
 
+Lemma ren_closed : forall ξ t, closed_tm 0 t -> t⟨ξ⟩ = t.
+Proof.
+  induction t; simpl; asimpl; auto.
+  - intro h; inversion h.
+  - intros; f_equal; auto.
+  - unfold is_true; rewrite Bool.andb_true_iff; intros (h1 & h2).
+    rewrite IHt1, IHt2; auto.
+  - unfold is_true; rewrite Bool.andb_true_iff; intros (h1 & h2).
+    rewrite IHt1, IHt2; auto.
+Qed.
 
 Lemma subst_closed : forall σ t, closed_tm 0 t -> t[σ] = t.
 Proof.
@@ -64,55 +74,102 @@ Proof.
     rewrite IHt1, IHt2; auto.
 Qed.
 
-
-Lemma tm_pattern_at_impl : forall P Q u, tm_pattern_at u (P ⇒ Q) = (tm_pattern_at u P) ⇒ (tm_pattern_at u Q).
+Lemma closed_n_tm : forall n, closed_tm 0 (n_tm n).
 Proof.
-  intros; reflexivity.
+  induction n; simpl; auto.
 Qed.
 
-Lemma tm_pattern_at_eq : forall t1 t2 u, tm_pattern_at u (t1 ≃ t2) = (tm_pattern_at_tm u t1) ≃ (tm_pattern_at_tm u t2).
+Hint Resolve closed_n_tm.
+
+Lemma closed_add1 : forall n1 n2, closed_tm 0 (Add n1 n2) -> closed_tm 0 n1.
 Proof.
-  intros; reflexivity.
+  induction n1; simpl; auto.
+  - intros ?; unfold is_true; repeat rewrite Bool.andb_true_iff; intuition.
+  - intros ?; unfold is_true; repeat rewrite Bool.andb_true_iff; intuition.
 Qed.
 
-Ltac patme u := (rewrite (tm_pattern_at_subst u); repeat rewrite tm_pattern_at_impl, tm_pattern_at_eq).
 
-
-Lemma trans_apply : forall Γ t1 t2 t3,
-    Γ ⊢ t1 ≃ t2 -> Γ ⊢ t2 ≃ t3 -> Γ ⊢ t1 ≃ t3.
+Lemma closed_add2 : forall n2 n1, closed_tm 0 (Add n1 n2) -> closed_tm 0 n2.
 Proof.
-  intros.
-  destruct (eq_dec_tm t1 t3); [subst; apply eq_refl|].
-  destruct (eq_dec_tm t2 t3); [subst; now auto|].
-  destruct (eq_dec_tm t1 t2); [subst; now auto|].
-  apply imp_elim with (P := t2 ≃ t3); auto.
-  apply imp_elim with (P := t1 ≃ t2); auto.
-  patme t3; apply forallt_elim.
-  patme t2; apply forallt_elim.
-  patme t1; apply forallt_elim.
+  induction n2; simpl; auto.
+  - intros ?; unfold is_true; repeat rewrite Bool.andb_true_iff; intuition.
+  - intros ?; unfold is_true; repeat rewrite Bool.andb_true_iff; intuition.
+  - intros ?; unfold is_true; repeat rewrite Bool.andb_true_iff; intuition.
+Qed.
+
+Hint Resolve closed_add2 closed_add1.
 
 Lemma eq_add : forall Γ k l,
     Γ ⊢ Add (n_tm k) (n_tm l) ≃ n_tm (k + l).
 Proof.
-  Search (_ + _).
   intros Γ k l; revert k Γ; induction l; intros; simpl; rewrite Nat.add_comm; simpl.
   - replace (Add (n_tm k) Z ≃ n_tm k) with ((Add (var_tm 0) Z ≃ (var_tm 0))[(n_tm k) ..; ids]) by (asimpl; simpl; auto).
     apply forallt_elim.
     apply plus_Z.
-  - apply imp_elim with (P := Succ (Add (n_tm k) (n_tm l)) ≃ Succ (n_tm (l+k))).
-    + apply imp_elim with (P := Add (n_tm k) (Succ (n_tm l)) ≃ Succ (Add (n_tm k) (n_tm l))).
-      -- Check eq_trans.
-         patme (Succ (n_tm (l+k))).
-         apply forallt_elim.
-         patme 
-         
-         pose (goal := Add (n_tm k) (Succ (n_tm l)) ≃ Succ (Add (n_tm k) (n_tm l))
-                           ⇒ Succ (Add (n_tm k) (n_tm l)) ≃ Succ (n_tm (l + k))
-                           ⇒ Add (n_tm k) (Succ (n_tm l)) ≃ Succ (n_tm (l + k))).
-         replace (Add (n_tm k) (Succ (n_tm l)) ≃ Succ (Add (n_tm k) (n_tm l))
-                      ⇒ Succ (Add (n_tm k) (n_tm l)) ≃ Succ (n_tm (l + k))
-                      ⇒ Add (n_tm k) (Succ (n_tm l)) ≃ Succ (n_tm (l + k))) with goal by reflexivity.
-         
+  - apply trans_apply with (t2 := Succ (Add (n_tm k) (n_tm l))).
+    + (* More replace hell... *)
+      replace (Add (n_tm k) (Succ (n_tm l)) ≃ Succ (Add (n_tm k) (n_tm l)))
+        with
+        (Add (n_tm k) (Succ (var_tm 0)) ≃ Succ (Add (n_tm k) (var_tm 0)))[(n_tm l)..; ids] by (asimpl; repeat rewrite subst_closed; auto).
+      apply forallt_elim.
+      replace (all Add (n_tm k) (Succ (var_tm 0)) ≃ Succ (Add (n_tm k) (var_tm 0)))
+        with
+        (all Add (var_tm 1) (Succ (var_tm 0)) ≃ Succ (Add (var_tm 1) (var_tm 0)))[(n_tm k)..;ids] by
+        (asimpl; repeat rewrite ren_closed; auto).
+      apply forallt_elim.
+      apply plus_S.
+    + apply succ_apply.
+      (* how did that happen? *)
+      replace (l + k) with (k + l) by (apply Nat.add_comm).
+      auto.
+Qed.
+
+Lemma tm_pattern_at_tm_mul_n : forall k t1 t2, tm_pattern_at_tm (Mult t1 t2) (n_tm k) = (n_tm k).
+Proof.
+  induction k; simpl; auto.
+  intros; f_equal; auto.
+Qed.
+
+Lemma eq_mult : forall Γ k l,
+    Γ ⊢ Mult (n_tm k) (n_tm l) ≃ n_tm (k * l).
+Proof.
+  intros Γ k l; revert k Γ; induction l; intros; simpl; rewrite Nat.mul_comm; simpl.
+  - replace (Mult (n_tm k) Z ≃ Z) with
+      (Mult (var_tm 0) Z ≃ Z)[(n_tm k)..; ids] by (asimpl; auto).
+    apply forallt_elim.
+    apply times_Z.
+  - Print derives.
+    apply trans_apply with (t2 := Add (n_tm k) (Mult (n_tm k) (n_tm l))).
+    + Check times_S.
+      replace
+        (Mult (n_tm k) (Succ (n_tm l)) ≃ Add (n_tm k) (Mult (n_tm k) (n_tm l)))
+        with
+        (Mult (n_tm k) (Succ (var_tm 0)) ≃ Add (n_tm k) (Mult (n_tm k) (var_tm 0)))[(n_tm l)..; ids] by (asimpl; repeat rewrite subst_closed; auto).
+      apply forallt_elim.
+      replace (all Mult (n_tm k) (Succ (var_tm 0)) ≃ Add (n_tm k) (Mult (n_tm k) (var_tm 0))) with (all Mult (var_tm 1) (Succ (var_tm 0)) ≃ Add (var_tm 1) (Mult (var_tm 1) (var_tm 0)))[(n_tm k)..; ids] by (asimpl; repeat rewrite subst_closed, ren_closed; repeat rewrite ren_closed; auto).
+      apply forallt_elim.
+      apply times_S.
+    + rewrite Nat.mul_comm.
+      pattac (Mult (n_tm k) (n_tm l)).
+      (* never do this! *)
+      (* unfold tm_pattern_at_tm. *)
+      rewrite tm_pattern_at_eq.
+      rewrite tm_pattern_at_tm_mul_n.
+      rewrite tm_pattern_at_tm_unfold.
+      edestruct (eq_dec_neq (Mult (n_tm k) (n_tm l)) (Add (n_tm k) (Mult (n_tm k) (n_tm l)))); [congruence |].
+      rewrite e; clear e.
+      clear x.
+      rewrite tm_pattern_at_tm_mul_n.
+      rewrite tm_pattern_at_tm_unfold.
+      rewrite eq_dec_eq.
+      eapply eq_subst.
+      -- apply sym_apply.
+         apply IHl.
+      -- asimpl.
+         repeat rewrite subst_closed; auto.
+         apply eq_add.
+Qed.
+      
 
 Lemma eq_norm : forall Γ vval t,
     closed_tm 0 t ->
@@ -123,27 +180,207 @@ Proof.
   - apply eq_refl.
   - inversion H.
     assert (h := IHt H1).
-    Locate "≃".
-    replace (Succ t ≃ Succ (n_tm (eval_tm vval t)))
-      with ((Succ t ≃ Succ (var_tm 0))[(n_tm (eval_tm vval t))..; ids]) by (asimpl; rewrite subst_closed; auto).
-    apply compr_elim.
-    eapply imp_elim with (P := t ∈ {{_ | Succ t ≃ Succ (var_tm 0) }}).
-    + replace (t ∈ ({{ _ | Succ t ≃ Succ (var_tm 0)}})
-                 ⇒ n_tm (eval_tm vval t) ∈ ({{ _ | Succ t ≃ Succ (var_tm 0)}})) with
-        ((t ∈ var_pred 0 ⇒ n_tm (eval_tm vval t) ∈ var_pred 0)[ids; {{ _ | Succ t ≃ Succ (var_tm 0)}}..]) by (asimpl; auto).
-      apply forallP_elim; auto.
-    + apply compr_intro.
-      asimpl; rewrite subst_closed; auto.
-      apply eq_refl.
-  - 
+    apply succ_apply; auto.
+  - apply trans_apply with (t2 := Add (n_tm (eval_tm vval t1)) (n_tm (eval_tm vval t2))); [ | apply eq_add].
+    replace (Add t1 t2 ≃ Add (n_tm (eval_tm vval t1)) (n_tm (eval_tm vval t2))) with
+      (Add t1 t2 ≃ Add (var_tm 0) (n_tm (eval_tm vval t2)))[(n_tm (eval_tm vval t1))..; ids] by (asimpl; repeat rewrite subst_closed; eauto).
+    eapply eq_subst; eauto; asimpl; repeat rewrite subst_closed; eauto.
+    replace (Add t1 t2 ≃ Add t1 (n_tm (eval_tm vval t2))) with
+      (Add t1 t2 ≃ Add t1 (var_tm 0))[(n_tm (eval_tm vval t2))..; ids] by (asimpl; repeat rewrite subst_closed; eauto).
+    eapply eq_subst; eauto; asimpl; repeat rewrite subst_closed; eauto.
+    apply eq_refl.
+  - apply trans_apply with (t2 := Mult (n_tm (eval_tm vval t1)) (n_tm (eval_tm vval t2))); [ | apply eq_mult].
+    replace (Mult t1 t2 ≃ Mult (n_tm (eval_tm vval t1)) (n_tm (eval_tm vval t2))) with
+      (Mult t1 t2 ≃ Mult (var_tm 0) (n_tm (eval_tm vval t2)))[(n_tm (eval_tm vval t1))..; ids] by (asimpl; repeat rewrite subst_closed; eauto).
+    eapply eq_subst; eauto; asimpl; repeat rewrite subst_closed; eauto.
+    replace (Mult t1 t2 ≃ Mult t1 (n_tm (eval_tm vval t2))) with
+      (Mult t1 t2 ≃ Mult t1 (var_tm 0))[(n_tm (eval_tm vval t2))..; ids] by (asimpl; repeat rewrite subst_closed; eauto).
+    eapply eq_subst; eauto; asimpl; repeat rewrite subst_closed; eauto.
+    apply eq_refl.
 Qed.
 
-Theorem eq_complete : forall t u,
+Theorem eq_complete : forall Γ t u,
     closed_tm 0 t ->
     closed_tm 0 u ->
     [] ⊧ t ≃ u ->
-    [] ⊢ t ≃ u.
+    Γ ⊢ t ≃ u.
 Proof.
   unfold "⊧".
   simpl.
+  intros.
+  assert (eval_tm id t = eval_tm id u).
+  - intros.
+    pattern (eval_tm id u) at 1.
+    eapply H1; eauto.
+    unfold validates; auto.
+  - apply trans_apply with (t2 := n_tm (eval_tm id u)).
+    + rewrite <- H2.
+      apply eq_norm; auto.
+    + apply sym_apply.
+      apply eq_norm; auto.
+      Unshelve.
+      unfold PVal.
+      apply (fun _ _ => False).
+Qed.
 
+
+Lemma neq_closed : forall n m Γ, n <> m -> Γ ⊢ n_tm n ≄ n_tm m.
+Proof.
+  induction n; induction m; simpl; intros; try congruence.
+  - apply imp_intro.
+    apply imp_elim with (P := (Succ (n_tm m) ≃ Z)).
+    + replace (Succ (n_tm m) ≄ Z) with (Succ (var_tm 0) ≄ Z)[(n_tm m)..;ids] by (asimpl; auto).
+      apply forallt_elim.
+      apply zero_S.
+    + apply sym_apply.
+      apply (axiom 0); auto.
+  - replace (Succ (n_tm n) ≄ Z) with (Succ (var_tm 0) ≄ Z)[(n_tm n)..;ids] by (asimpl; auto).
+    apply forallt_elim.
+    apply zero_S.
+  - apply imp_intro.
+    apply imp_elim with (P := (n_tm n) ≃ (n_tm m)).
+    + apply IHn; auto.
+    + eapply imp_elim; [| apply (axiom 0); simpl; eauto].
+      Check inj_S.
+      replace (Succ (n_tm n) ≃ Succ (n_tm m) ⇒ n_tm n ≃ n_tm m)
+        with (Succ (n_tm n) ≃ Succ (var_tm 0) ⇒ n_tm n ≃ var_tm 0)[(n_tm m)..; ids]
+        by (asimpl; rewrite subst_closed; auto).
+      apply forallt_elim.
+      replace (all Succ (n_tm n) ≃ Succ (var_tm 0) ⇒ n_tm n ≃ var_tm 0) with (all Succ (var_tm 1) ≃ Succ (var_tm 0) ⇒ var_tm 1 ≃ var_tm 0)[(n_tm n)..; ids] by (asimpl; rewrite ren_closed; auto).
+      apply forallt_elim.
+      apply inj_S.
+Qed.
+
+
+(* Ooof this is not trivial from the other one *)
+Theorem neq_complete : forall Γ t u,
+    closed_tm 0 t ->
+    closed_tm 0 u ->
+    [] ⊧ t ≄ u ->
+    Γ ⊢ t ≄ u.
+Proof.
+  intros Γ t u cl_t cl_u neq_sem.
+  apply imp_intro.
+  apply imp_elim with (P := (n_tm (eval_tm id t)) ≃ (n_tm (eval_tm id u))).
+  - assert (eval_tm id t <> eval_tm id u).    
+    + unfold "⊧" in *.
+      simpl in neq_sem.
+      intro.
+      eapply neq_sem; unfold validates; auto.
+      -- rewrite H; auto.
+      -- exact 0.
+    + apply neq_closed; auto.
+  - apply trans_apply with (t2 := t) ; [apply sym_apply; apply eq_norm; auto|].
+    apply trans_apply with (t2 := u); [| apply eq_norm; auto].
+    apply (axiom 0); auto.
+    Unshelve.
+    unfold PVal.
+    apply (fun _ _ => False).
+Qed.
+
+Lemma subst_lift_tm : forall (t : tm) ξ, t[ξ >> var_tm] = t⟨ξ⟩.
+Proof.
+  induction t; intros; asimpl; try rewrite IHt; auto.
+  - rewrite IHt1, IHt2; auto.
+  - rewrite IHt1, IHt2; auto.
+Qed.
+
+Lemma subst_lift : forall (P : prop) (ξ : fin -> fin) (σ : fin -> tm), P[ξ >> σ; var_pred] = (P ⟨ξ; id⟩ [σ; ids]).
+Proof.
+  intros.
+  asimpl.
+  auto.
+Qed.
+
+Lemma subst_lift' : forall (P : prop) ξ, P[ξ >> var_tm; var_pred] = P ⟨ξ; id⟩.
+Proof.
+  intros.
+  replace (P ⟨ξ; id⟩) with (P ⟨ξ; id⟩[var_tm; ids]) by (asimpl; auto).
+  apply subst_lift.
+Qed.
+
+Lemma exfalso_apply : forall Γ P, Γ ⊢ ⊥ -> Γ ⊢ P.
+Proof.
+  intros Γ P fls.
+  replace P with (P⟨↑; ids⟩ [(var_tm 0)..; ids]) by (asimpl; unfold idsRen; asimpl; auto).
+  apply compr_elim.
+  replace (var_tm 0 ∈ {{_ | P ⟨↑; ids⟩ }}) with
+    (var_tm 0 ∈ {{_ | P ⟨↑ >> ↑; ids⟩ }})[(var_tm 0)..; ids]
+    by (asimpl;
+       unfold idsRen;
+       asimpl;
+        rewrite subst_lift'; auto).
+  apply forallt_elim.
+  
+  replace (all var_tm 0 ∈ {{_ | P ⟨↑ >> ↑ ; ids⟩ }}) with
+    (all var_tm 0 ∈ var_pred 0)[ids; {{_ | P ⟨↑ ; ids⟩ }}..] by (asimpl; auto).
+  apply forallP_elim; auto.
+Qed.
+
+Notation "P ∧ Q" := (FORALL (P⟨id; ↑⟩ ⇒ Q⟨id; ↑⟩ ⇒ all (var_tm 0) ∈ (var_pred 0)) ⇒ all (var_tm 0) ∈ (var_pred 0)) (at level 25).
+
+Notation "P ∨ Q" := (FORALL (P⟨id; ↑⟩ ⇒ all (var_tm 0) ∈ (var_pred 0)) ⇒
+                            (Q⟨id; ↑⟩ ⇒ all (var_tm 0) ∈ (var_pred 0)) ⇒
+                            all (var_tm 0) ∈ (var_pred 0)) (at level 25).
+
+
+Class complete Γ P := { reflect : Γ ⊧ P -> Γ ⊢ P }.
+
+Lemma superweak : forall Γ P, nil ⊢ P -> Γ ⊢ P.
+Proof.
+  induction Γ; auto.
+  intros.
+  apply weakening; auto.
+Qed.
+
+Lemma reflect_closed {P : prop} [cp : complete nil P] : forall Γ, [] ⊧ P -> Γ ⊢ P.
+  intros; apply superweak.
+  apply reflect; auto.
+Qed.
+
+Instance complete_eq (t u : tm) : closed_tm 0 t -> closed_tm 0 u -> complete nil (t ≃ u).
+intros; constructor; intros; apply eq_complete; auto.
+Qed.
+
+Instance complete_neq (t u : tm) : closed_tm 0 t -> closed_tm 0 u -> complete nil (t ≄ u).
+intros; constructor; intros; apply neq_complete; auto.
+Qed.
+
+(* Useless on its own, but may find use later. *)
+Instance complete_false : complete nil ⊥.
+constructor; unfold "⊧"; simpl; intros.
+exfalso.
+apply (H (fun _ _ => False) (fun _ => 0)); unfold validates; auto.
+exact 0.
+Qed.
+
+(* This does *not* hold with the current definition of completeness *)
+Instance complete_imp {Γ P Q} {cq : complete (P::Γ) Q} : complete Γ (P ⇒ Q).
+constructor; intros.
+apply imp_intro.
+apply reflect.
+unfold "⊧" in *; simpl in *; intros.
+apply H.
+- inversion H0; subst; auto.
+- inversion H0; auto.
+Qed.
+
+Print "⊧".
+
+Definition bot_pval : PVal := fun _ _ => False.
+Definition bot_vval : VVal := fun _ => 0.
+
+Theorem ex_refl :
+  forall P, [] ⊢ ∃ P -> exists n, eval_prop bot_pval (n, bot_vval) P.
+Proof.
+  intros.
+  Check soundness.
+  assert (h : [] ⊧ ∃ P) by (apply soundness; auto).
+  unfold "⊧" in *; simpl in *.
+  assert (val_nil : validates bot_pval bot_vval nil) by (unfold validates; auto).
+  apply (h bot_pval bot_vval val_nil (fun _ => exists n, eval_prop bot_pval (n, bot_vval) P)); [ | exact 0].
+  intros.
+  exists n.
+  rewrite eval_ren in H0; asimpl in *.
+  auto.
+Qed.
